current/Main.v
@@ -1,74 +1,57 @@
 Require Import cliqueColorable.    
+ 
+Ltac inSet :=
+  match goal with
+      |H:Ensembles.In _ (Add _ ?x ?y) ?z |- _ => inv H
+      |H:Ensembles.In _ (Singleton _ ?x) ?y |- _ => inv H
+  end. 
 
 Theorem validEnvDomainUnique : forall Gamma C eta' eta i U, 
-                                 valid Gamma C i eta' eta ->
-                                 (forall x, Ensembles.In _ U x -> x > 3 * i + 2) -> 
+                                 setVertices Gamma C i eta' eta ->
+                                 (forall x, Ensembles.In _ U x -> x < 3 * i) -> 
                                  genericUnique U (fun a => match a with (x,y) => x end) eta'. 
 Proof.
   intros. genDeps {{ U }}. induction H; intros. 
-  {constructor. constructor. constructor. eapply IHvalid. intros. inv H3.
-   inv H4. inv H1. apply H2 in H3. omega. inv H3. omega. inv H1. omega. inv H4. omega.
-   intros c. inv c. inv H3. apply H2 in H1. omega. inv H1. omega. inv H3. omega. 
-   intros c. inv c. apply H2 in H3. omega. inv H3. omega. intros c. apply H2 in c. omega. }
-  {constructor. constructor. constructor. eapply IHvalid. intros. inv H3.
-   inv H4. inv H1. apply H2 in H3. omega. inv H3. omega. inv H1. omega. inv H4. omega.
-   intros c. inv c. inv H3. apply H2 in H1. omega. inv H1. omega. inv H3. omega. 
-   intros c. inv c. apply H2 in H3. omega. inv H3. omega. intros c. apply H2 in c. omega. }
+  {constructor. constructor. constructor. eapply IHsetVertices. intros. inSet. inSet.
+   inSet. apply H1 in H3. omega. inSet. omega. inSet. omega. inSet. omega. intros c. inSet. 
+   inSet. apply H1 in H3. omega. inSet. omega. inSet. omega. intros c. inSet. apply H1 in H2. 
+   omega. inSet. omega. intros c. apply H1 in c. omega. }
+  {constructor. constructor. constructor. eapply IHsetVertices. intros. inSet. inSet.
+   inSet. apply H1 in H3. omega. inSet. omega. inSet. omega. inSet. omega. intros c. inSet. 
+   inSet. apply H1 in H3. omega. inSet. omega. inSet. omega. intros c. inSet. apply H1 in H2. 
+   omega. inSet. omega. intros c. apply H1 in c. omega. }
   {constructor. }
 Qed. 
 
-Theorem KColorNPC : forall Gamma Delta F C eta G eta' S1 S2 S3 S4 U,
-                      reduce Gamma Delta F C G -> uniqueLockstep S1 S2 S3 S4 Gamma ->
-                      valid Gamma C 1 eta' eta -> genericUnique U (fun x => x) Delta -> 
+Theorem KColorNPC : forall Gamma Delta F C eta G eta' U,
+                      reduce Gamma Delta F C G -> 
+                      valid Gamma C F eta' eta -> genericUnique U (fun x => x) Delta -> 
                       (SAT' eta F <-> coloring eta' G C).
 Proof. 
   intros. inv H. split; intros. 
-  {constructor. admit. constructor. copy H1. 
-   apply validEnvDomainUnique with (U:=Empty_set _) in H1. Focus 2. intros. 
-   inv H7. eapply cliqueColorable; eauto. admit. }
+  {constructor. admit. constructor. inv H0. eapply colorWeakening. eapply cliqueColorable; eauto. 
+   admit. }
   {Admitted. 
 
 
-Theorem buildCtxtUnique : forall n Gamma Delta U, 
-                            (Gamma, Delta) = buildCtxt n -> 
-                            (forall x, Ensembles.In vvar U x -> x > n) -> 
+Theorem buildCtxtUnique : forall i n Gamma Delta U, 
+                            buildCtxt n i Gamma Delta -> 
+                            (forall x, Ensembles.In vvar U x -> x < i) -> 
                             genericUnique U (fun x=> x) Delta. 
 Proof.
-  induction n; intros. 
-  {simpl in *. inv H. constructor. }
-  {simpl in *. destruct (buildCtxt n). invertTupEq. constructor.
-   eapply IHn; eauto. intros. inv H. apply H0 in H1. omega. inv H1. omega. 
-   intros c. apply H0 in c. omega. }
-Qed. 
-
-Theorem buildCtxtUniqueLS : forall n Gamma Delta S1 S2 S3 S4, 
-                              (Gamma, Delta) = buildCtxt n -> 
-                              (forall x, Ensembles.In vvar S1 x -> x > n) ->
-                              (forall x, Ensembles.In vvar S2 x -> x > 3*n) ->
-                              (forall x, Ensembles.In vvar S3 x -> x > 3*n+1) ->
-                              (forall x, Ensembles.In vvar S4 x -> x > 3*n+2) ->
-                              uniqueLockstep S1 S2 S3 S4 Gamma.
-Proof.
-  induction n; intros. 
-  {simpl in *. invertTupEq. repeat econstructor. }
-  {simpl in *. destruct (buildCtxt n) eqn:eq. invertTupEq. constructor. 
-   eapply IHn; auto. intros; inv H;[apply H0 in H4; omega|inv H4;omega].
-   intros; inv H; [apply H1 in H4; omega|inv H4;omega].  
-   intros; inv H;[apply H2 in H4; omega|inv H4;omega]. 
-   intros; inv H;[apply H3 in H4; omega|inv H4;omega]. 
-   intros c. apply H0 in c. omega. intros c. apply H1 in c. omega. intros c. 
-   apply H2 in c. omega. intros c. apply H3 in c. omega. }
+  intros. generalize dependent U. induction H; intros. 
+  {constructor. eapply IHbuildCtxt. intros. inSet. apply H0 in H2. 
+   auto. inSet. omega. intros c. apply H0 in c. omega. }
+  {constructor. }
 Qed. 
 
 Theorem KColorNPCTopLevel : forall Gamma Delta F n G eta eta', 
-                              (Gamma, Delta) = buildCtxt n ->
-                              reduce Gamma Delta F (n+1) G -> valid Gamma (n+1) 1 eta' eta ->
+                              buildCtxt n 0 Gamma Delta ->
+                              reduce Gamma Delta F (n+1) G -> valid Gamma (n+1) F eta' eta ->
                               (SAT' eta F <-> coloring eta' G (n+1)). 
 Proof.
-  intros. copy H. apply buildCtxtUnique with (U:=Empty_set _) in H. Focus 2. intros. 
-  inv H3. eapply buildCtxtUniqueLS with (S1:=Empty_set _)(S2:=Empty_set _)
-          (S3:=Empty_set _)(S4:=Empty_set _) in H2; try solve[intros c1 c2; inv c2].
-  eapply KColorNPC in H0; eauto. 
+  intros. apply buildCtxtUnique with (U:=Empty_set _) in H. Focus 2. intros. 
+  inv H2. eapply KColorNPC in H0; eauto. 
 Qed. 
 
 
