current/cliqueColorable.v
@@ -1,70 +1,53 @@
 Require Export ThreeSatReduction.  
 
-Theorem edgesNeq : forall eta' eta Gamma C i u U u1 S1 S2 S3 S4, 
+Theorem edgesNeq : forall eta' eta Gamma C i u u1, 
                      u <> u1 -> In (u,3*u,3*u+1,3*u+2) Gamma -> In (u1,3*u1,3*u1+1,3*u1+2) Gamma ->
-                     valid Gamma C i eta' eta -> uniqueLockstep S1 S2 S3 S4 Gamma ->
-                     genericUnique U (fun a=>match a with (x,y) => x end) eta' ->
+                     setVertices Gamma C i eta' eta -> 
                      exists c1 c2, In (3*u+2,c1) eta' /\ In (3*u1+2, c2) eta' /\ c1 <> c2 /\
                               c1 <= C /\ c2 <= C. 
 Proof.
-  intros. genDeps {{ u;u1;S1;S2;S3;S4;U }}. induction H2; intros.
-  {inv H1.  
-   {inv H6. 
-    {invertTupEq. omega. }
-    {invertTupEq. inv H3. copy H2. eapply InValid in H2; eauto. invertHyp. 
-     econstructor. econstructor. split. simpl. repeat right. eauto. split. 
-     simpl. auto. invUnique. eapply ltValid in H13; eauto.
-     split. omega. split; auto. }
-   }
-   {inv H6. 
-    {invUnique. invertTupEq. exists (S i). copy H2. eapply InValid in H2; eauto. invertHyp. exists x. 
-     split; simpl; auto. split. auto. split; auto. eapply ltValid in H2; eauto. omega. }
-    {invUnique. eapply IHvalid in H7; eauto. invertHyp. exists x0. exists x. simpl. split; auto. }
-   }
+  intros. genDeps {{ u;u1 }}. induction H2; intros.
+  {inCons. 
+   {inCons. invertTupEq. omega. invertTupEq. copy H2. eapply InSetVertices in H2; eauto. 
+    invertHyp. eapply geSetVertices in H1; eauto. exists u0. exists x. split. simpl. 
+    auto. split. simpl. auto. split; auto. omega. split; auto. omega. }
+   {inCons. invertTupEq. copy H2. eapply InSetVertices in H2; eauto. 
+    invertHyp. eapply geSetVertices in H1; eauto. exists x. exists u1. split. simpl. auto. split. 
+    simpl. auto. split. omega. split; auto. omega. eapply IHsetVertices in H0; eauto. 
+    invertHyp. exists x. exists x0. split. simpl. auto. split. simpl. auto. auto. }
   }
-  {inv H1.  
-   {inv H6. 
-    {invertTupEq. omega. }
-    {invertTupEq. inv H3. copy H2. eapply InValid in H2; eauto. invertHyp. 
-     econstructor. econstructor. split. simpl. repeat right. eauto. split. 
-     simpl. auto. invUnique. eapply ltValid in H13; eauto.
-     split. omega. split; auto. }
-   }
-   {inv H6. 
-    {invUnique. invertTupEq. exists (S i). copy H2. eapply InValid in H2; eauto. invertHyp. exists x. 
-     split; simpl; auto. split. auto. split; auto. eapply ltValid in H2; eauto. omega. }
-    {invUnique. eapply IHvalid in H7; eauto. invertHyp. exists x0. exists x. simpl. split; auto. }
-   }
+  {inCons. 
+   {inCons. invertTupEq. omega. invertTupEq. copy H2. eapply InSetVertices in H2; eauto. 
+    invertHyp. eapply geSetVertices in H1; eauto. exists u0. exists x. split. simpl. 
+    auto. split. simpl. auto. split; auto. omega. split; auto. omega. }
+   {inCons. invertTupEq. copy H2. eapply InSetVertices in H2; eauto. 
+    invertHyp. eapply geSetVertices in H1; eauto. exists x. exists u1. split. simpl. auto. split. 
+    simpl. auto. split. omega. split; auto. omega. eapply IHsetVertices in H0; eauto. 
+    invertHyp. exists x. exists x0. split. simpl. auto. split. simpl. auto. auto. }
   }
   {inv H0. }
 Qed. 
 
-Theorem connectXColorable : forall Gamma Delta G C eta eta' U u S1 S2 S3 S4, 
-                              uniqueLockstep S1 S2 S3 S4 Gamma -> 
-                              ~In u Delta -> valid Gamma C 1 eta' eta -> In (u,3*u,3*u+1,3*u+2) Gamma ->
-                              genericUnique U (fun a=>match a with (x,y) => x end) eta' ->
+Theorem connectXColorable : forall Gamma Delta G C eta eta' u, 
+                              ~In u Delta -> setVertices Gamma C 0 eta' eta -> In (u,3*u,3*u+1,3*u+2) Gamma ->
                               connectX Gamma Delta (3*u+2) G -> coloring eta' G C. 
 Proof.
-  intros. genDeps {{ eta; C; eta'}}. remember (3*u+2). induction H4; intros. 
+  intros. genDeps {{ eta; C; eta'}}. remember (3*u+2). induction H2; intros. 
   {constructor. } 
-  {subst. copy H5. eapply validUnique with (S := Empty_set _) in H5. 
-   destruct(eq_nat_dec u u0). 
-   {subst. simpl in H2. exfalso. apply H0. simpl. auto. }
-   {copy H6. eapply edgesNeq in H6; eauto. invertHyp. econstructor; eauto.
-    eapply IHconnectX; eauto. intros c. apply H0. simpl. right. auto. }
-   intros. inv H7. 
+  {subst. destruct(eq_nat_dec u u0). 
+   {subst. exfalso. apply H. simpl. auto. }
+   {copy H3. eapply edgesNeq in H3; eauto. invertHyp. econstructor; eauto.
+    eapply IHconnectX; eauto. intros c. apply H. simpl. right. auto. }
   }
 Qed. 
-
-Theorem cliqueColorable : forall Gamma eta Delta C G eta' U S1 S2 S3 S4 S5, 
-                            valid Gamma C 1 eta' eta -> 
-                            uniqueLockstep S1 S2 S3 S4 Gamma ->
+ 
+Theorem cliqueColorable : forall Gamma eta Delta C G eta' S5, 
+                            setVertices Gamma C 0 eta' eta -> 
                             genericUnique S5 (fun x => x) Delta -> 
-                            genericUnique U (fun a=>match a with (x,y) => x end) eta' ->
                             clique Gamma Delta G -> coloring eta' G C. 
 Proof.
-  intros. genDeps {{ eta; C; U }}. induction H3; intros; auto. 
-  {constructor. eapply IHclique; eauto. inv H1. eapply genericUniqueSubset; eauto. 
-   eapply connectXColorable; eauto. inv H1. eapply genericUniqueNotIn. 
+  intros. genDeps {{ eta; C }}. induction H1; intros; auto. 
+  {constructor. eapply IHclique; eauto. inv H0. eapply genericUniqueSubset; eauto. 
+   eapply connectXColorable; eauto. inv H0. eapply genericUniqueNotIn. 
    Focus 2. eauto. simpl. apply Union_intror. constructor. }
 Qed. 
